Remove dependency to oldlibs for Group

theories/algebra/Group.ec
@@ -234,6 +234,7 @@ proof.
 move=> mn x y; move: (mn x) (mn y).
 by move=> [kx ->] [ky ->]; rewrite -!expD addrC.
 qed.
+
 end Group.
 
 (* ==================================================================== *)
@@ -250,7 +251,7 @@ clone include Group
   with type group <- group,
          op e     <- e    ,
          op ( * ) <- ( * ),
-         op inv   <- inv  
+         op inv   <- inv
   proof mulc1, mulcV
   rename "invM" as "invM_com".
 
@@ -448,8 +449,10 @@ type exp.
 
 axiom prime_order : prime order.
 
-clone import ZModP.ZModField as ZModE with type zmod <- exp, op p <- order
+clone ZModP.ZModField as ZModE with type zmod <- exp, op p <- order
   proof prime_p by apply: prime_order.
+
+import ZModE.
 
 (* -------------------------------------------------------------------- *)
 op (^)  (x : group) (k : exp) = x ^ (asint k)
@@ -535,10 +538,107 @@ lemma expV (x : group) (k : exp) :
   unit k => root k (x ^ k) = x.
 proof. by rewrite -expM=> /ZModpRing.mulrV ->; exact/exp1. qed.
 
+lemma expgK' (x : group) : x = g ^ log x by rewrite expgK.
+
+lemma nosmt logg1 : loge g = one by rewrite -exp1 loggK.
+
+lemma logrzM' (x : group) (a : exp) : loge (x ^ a) = loge x * a
+  by rewrite logrzM; algebra.
+
+(* Isn't it just inj? *)
+lemma nosmt log_bij (x y : group) : x = y <=> loge x = loge y.
+proof.
+split => [/#|]; suff mono_exp : forall x, exists (kx : exp), x = g ^ kx
+  by move: (mono_exp x) (mono_exp y) => [kx ->] [ky ->]; rewrite !loggK => ->.
+move => {x y} x; case: (monogenous x) => k -> {x}; exists (inzmod k).
+pose kr := k %% order; have -> : g ^ k = g ^ kr
+  by rewrite (divz_eq k order) expD mulrC expM expg_order expc1 mul1c.
+suff: kr = asint (inzmod k) by smt().
+by rewrite /kr /inzmod /asint Sub.insubdK; smt(gt0_order ltz_pmod modz_ge0).
+qed.
+
+lemma nosmt pow_bij (x y : exp) : x = y <=> g ^ x = g ^ y
+  by rewrite -loggK -(loggK y) !expgK -log_bij.
+
+lemma nosmt inv_def (a : group) : inv a = g ^ (-loge a)
+  by rewrite log_bij logrV loggK.
+
+lemma nosmt div_def (a b : group): g ^ (loge a - loge b) = a / b
+  by rewrite log_bij logDrN loggK.
+
+lemma nosmt g_neq0 : g ^ zero <> g
+  by rewrite -{2}exp1 -pow_bij; smt(ZModpField.unitr1).
+
+lemma mulN (x : group) : x * inv x = g ^ zero by rewrite mulcV -(exp0 g).
+
+hint rewrite Ring.inj_algebra : expgK'. (* reverse equality? *)
+hint rewrite Ring.rw_algebra : logg1 logrzM' logDr log_bij.
+
+abstract theory FDistr.
+
+import ZModE.DZmodP.
+
+(* distribution *)
+op dt : exp distr = dunifin.
+
+require import Distr.
+
+lemma dt_fu: is_full dt by exact dunifin_fu.
+
+lemma dt1E (s : exp) : mu1 dt s = (1%r / order%r)%Real
+  by rewrite dunifin1E cardE.
+
+lemma dt_ll: is_lossless dt by exact dunifin_ll.
+
+lemma dt_funi: is_funiform dt.
+proof. by move=> ??;rewrite !dt1E. qed.
+
+lemma supp (s : exp) : 0%r < mu1 dt s.
+proof.
+rewrite dt1E StdOrder.RealOrder.ltr_pdivl_mulr; 1: by smt(order_gt0).
+by rewrite StdBigop.Bigreal.Num.Domain.mul0r StdOrder.RealOrder.ltr01.
+qed.
+
+hint exact random : dt_fu dt_ll dt_funi.
+
+abstract theory Cost.
+  op cdt : {int | 0 <= cdt } as ge0_cdt.
+  schema cost_dt `{P}: cost [P: dt] = N cdt.
+  hint simplify cost_dt.
+end Cost.
+
+end FDistr.
+
+abstract theory Cost.
+  op cgpow : int.
+  op cgmul: int.
+  op cgdiv: int.
+  op cgeq : int.
+  axiom ge0_cg : 0 <= cgpow /\ 0 <= cgmul /\ 0 <= cgdiv /\ 0 <= cgeq.
+
+  schema cost_gen `{P} : cost [P:g] = '0.
+
+  schema cost_pow `{P} {g:group, x:exp} :
+    cost[P: g ^ x] = cost[P:g] + cost[P:x] + N cgpow.
+
+  schema cost_gmul `{P} {g1 g2:group} :
+    cost[P:g1 * g2] = cost[P:g1] + cost[P:g2] + N cgmul.
+
+  schema cost_geq  `{P} {g1 g2:group} :
+    cost[P:g1 = g2] = cost[P:g1] + cost[P:g2] + N cgeq.
+
+  schema cost_gdiv `{P} {g1 g2:group} :
+    cost[P:g1 / g2] = cost[P:g1] + cost[P:g2] + N cgdiv.
+
+  hint simplify cost_gen, cost_pow, cost_gmul, cost_gdiv, cost_geq.
+end Cost.
+
 end PowZMod.
+
 end CyclicGroup.
 
 (* ==================================================================== *)
+
 abstract theory ZModPCyclic.
 type zmod.
 
@@ -578,4 +678,5 @@ move=> x; exists (asint x) => @/g; rewrite {1}(intmul_asint x).
 rewrite /intmul /(^) ltrNge ge0_asint /=.
 by rewrite AddMonoid.iteropE /(^+) ger0_norm ?ge0_asint.
 qed.
+
 end ZModPCyclic.
